describe add

Cslib/Computability/Machines/MultiTapeTuring/CopyRoutine.lean
@@ -12,6 +12,7 @@ import Cslib.Foundations.Data.RelatesInSteps
 public import Cslib.Computability.Machines.MultiTapeTuring.Basic
 public import Cslib.Computability.Machines.MultiTapeTuring.ListEncoding
 public import Cslib.Computability.Machines.MultiTapeTuring.HeadStats
+public import Cslib.Computability.Machines.MultiTapeTuring.WithTapes
 
 -- TODO create a "common file"
 import Cslib.Computability.Machines.SingleTapeTuring.Basic
@@ -22,22 +23,36 @@ namespace Routines
 
 variable [Inhabited α] [Fintype α]
 
-public def copy : MultiTapeTM 2 (WithSep α) where
+public def copy₁ : MultiTapeTM 2 (WithSep α) where
   Λ := PUnit
   q₀ := 0
   M _ syms := sorry
 
 @[simp]
-public lemma copy_eval_list {w : List α} {ls₁ ls₂ : List (List α)} :
-  copy.eval_list [w :: ls₁, ls₂].get = Part.some [w :: ls₁, w :: ls₂].get := by
+public lemma copy₁_eval_list {w : List α} {ls₁ ls₂ : List (List α)} :
+  copy₁.eval_list [w :: ls₁, ls₂].get = Part.some [w :: ls₁, w :: ls₂].get := by
   sorry
 
-public lemma copy_evalWithStats {w : List α} {ls₁ ls₂ : List (List α)} :
-  copy.evalWithStats_list #v[w :: ls₁, ls₂].get =
+public def copy {k : ℕ} (i j : Fin k.succ) (h_neq : i ≠ j := by decide) :
+  MultiTapeTM k.succ (WithSep α) :=
+  copy₁.with_tapes #v[i, j] (h_le := by omega)
+
+@[simp, grind =]
+public lemma copy_eval_list
+  {k : ℕ} {i j : Fin k.succ} {h_neq : i ≠ j}
+  {tapes : Fin k.succ → List (List α)}
+  {h_tapes_i : tapes i ≠ []} :
+  (copy i j (h_neq := h_neq)).eval_list tapes = Part.some
+    (Function.update tapes j (((tapes i).head h_tapes_i) :: (tapes j))) := by
+  sorry
+
+public lemma copy₁_evalWithStats {w : List α} {ls₁ ls₂ : List (List α)} :
+  copy₁.evalWithStats_list #v[w :: ls₁, ls₂].get =
     .some (
       [w :: ls₁, w :: ls₂].get,
       [⟨-1, w.length, 0, by omega⟩, ⟨-w.length - 2, 0, -w.length - 1, by omega⟩].get) := by
   sorry
+
 
 -- TODO at some point, we might not want exact stats but rather an upper bound.
 -- Can this be made compatible with using equality?
