Cslib/Computability/Machines/MultiTapeTuring/EqualRoutine.lean
@@ -12,6 +12,7 @@ import Cslib.Foundations.Data.RelatesInSteps
 public import Cslib.Computability.Machines.MultiTapeTuring.Basic
 public import Cslib.Computability.Machines.MultiTapeTuring.ListEncoding
 public import Cslib.Computability.Machines.MultiTapeTuring.HeadStats
+public import Cslib.Computability.Machines.MultiTapeTuring.WithTapes
 
 namespace Turing
 
@@ -20,18 +21,35 @@ namespace Routines
 --- A 3-tape Turing machine that pushes the new word "1"
 --- to the third tape if the first words on the first and second tape are the same
 --- and otherwise pushes the empty word to the third tape.
-public def eq : MultiTapeTM 3 (WithSep OneTwo) where
+public def eq₀ : MultiTapeTM 3 (WithSep OneTwo) where
   Λ := PUnit
   q₀ := 0
   M _ syms := sorry
 
 @[simp]
-public theorem eq_eval_list (w₁ w₂ : List OneTwo) (ws₁ ws₂ ws₃ : List (List OneTwo)) :
-  eq.eval_list [w₁ :: ws₁, w₂ :: ws₂, ws₃].get =
+public theorem eq₀_eval_list (w₁ w₂ : List OneTwo) (ws₁ ws₂ ws₃ : List (List OneTwo)) :
+  eq₀.eval_list [w₁ :: ws₁, w₂ :: ws₂, ws₃].get =
     Part.some (if w₁ = w₂ then
       [w₁ :: ws₁, w₂ :: ws₂, [.one] :: ws₃].get
     else
       [w₁ :: ws₁, w₂ :: ws₂, [] :: ws₃].get) := by
+  sorry
+
+public def eq {k : ℕ} (q s t : Fin k)
+  (h_neq : q ≠ s := by decide) (h_neq' : q ≠ t := by decide) (h_neq'' : s ≠ t := by decide) :
+  MultiTapeTM k (WithSep OneTwo) :=
+  eq₀.with_tapes #v[q, s, t] (h_le := by omega)
+
+@[simp, grind =]
+public theorem eq_eval_list {k : ℕ} {q s t : Fin k}
+  {h_neq : q ≠ s} {h_neq' : q ≠ t} {h_neq'' : s ≠ t}
+  {tapes : Fin k → List (List OneTwo)} {h_q_nonempty : tapes q ≠ []} {h_s_nonempty : tapes s ≠ []} :
+  (eq q s t (h_neq := h_neq) (h_neq' := h_neq') (h_neq'' := h_neq'')).eval_list tapes =
+    Part.some (Function.update tapes t
+      ((if (tapes q).head h_q_nonempty = (tapes s).head h_s_nonempty then
+        [.one]
+      else
+        []) :: (tapes t))) := by
   sorry
 
 end Routines
