Cslib/Computability/Machines/MultiTapeTuring/IteCombinator.lean
@@ -22,19 +22,20 @@ variable {k : ℕ}
 
 --- Repeatedly run a sub routine as long as a condition on the symbol
 --- at the first head is true.
-public def ite (tm₁ tm₂ : MultiTapeTM k.succ (WithSep α)) :
-    MultiTapeTM k.succ (WithSep α) where
+public def ite (i : Fin k) (tm₁ tm₂ : MultiTapeTM k (WithSep α)) :
+    MultiTapeTM k (WithSep α) where
   Λ := PUnit
   q₀ := 0
   M _ syms := sorry
 
-@[simp]
+@[simp, grind =]
 public theorem ite_eval
-  (tm₁ tm₂ : MultiTapeTM k.succ (WithSep α))
-  (tapes : Fin k.succ → List (List α))
-  (h_nonempty : tapes 0 ≠ []) :
-  (ite tm₁ tm₂).eval_list tapes =
-    if (tapes 0).head h_nonempty = [] then tm₂.eval_list tapes else tm₁.eval_list tapes := by
+  {i : Fin k}
+  {tm₁ tm₂ : MultiTapeTM k (WithSep α)}
+  {tapes : Fin k → List (List α)}
+  {h_nonempty : tapes i ≠ []} :
+  (ite i tm₁ tm₂).eval_list tapes =
+    if (tapes i).head h_nonempty = [] then tm₂.eval_list tapes else tm₁.eval_list tapes := by
   sorry
 
 end Routines
