Cslib/Computability/Machines/MultiTapeTuring/PushRoutine.lean
@@ -11,6 +11,7 @@ import Cslib.Foundations.Data.RelatesInSteps
 
 public import Cslib.Computability.Machines.MultiTapeTuring.Basic
 public import Cslib.Computability.Machines.MultiTapeTuring.ListEncoding
+public import Cslib.Computability.Machines.MultiTapeTuring.WithTapes
 
 -- TODO create a "common file"
 import Cslib.Computability.Machines.SingleTapeTuring.Basic
@@ -21,18 +22,27 @@ namespace Routines
 
 variable [Inhabited α] [Fintype α]
 
-public def push (w : List α) : MultiTapeTM 1 (WithSep α) where
+public def push₁ (w : List α) : MultiTapeTM 1 (WithSep α) where
   Λ := PUnit
   q₀ := 0
   M _ syms := sorry
 
 @[simp]
-public lemma push_eval_list {w : List α} {ls : List (List α)} :
-  (push w).eval_list [ls].get = .some [w :: ls].get := by
+public lemma push₁_eval_list {w : List α} {ls : List (List α)} :
+  (push₁ w).eval_list [ls].get = .some [w :: ls].get := by
   sorry
 
-public lemma push_evalWithStats_list {w : List α} {ls : List (List α)} :
-  (push w).evalWithStats_list #v[ls].get =
+public def push {k : ℕ} (i : Fin k.succ) (w : List α) : MultiTapeTM k.succ (WithSep α) :=
+  (push₁ w).with_tapes #v[i] (h_le := by omega)
+
+@[simp, grind =]
+public theorem push_eval_list {k : ℕ} (i : Fin k.succ) (w : List α) (tapes : Fin k.succ → List (List α)) :
+  (push i w).eval_list tapes =
+    .some (Function.update tapes i (w :: (tapes i))) := by
+  sorry
+
+public lemma push₁_evalWithStats_list {w : List α} {ls : List (List α)} :
+  (push₁ w).evalWithStats_list #v[ls].get =
     .some (
       [w :: ls].get,
       [⟨-w.length - 1, 0, -w.length - 1, by omega⟩].get) := by
