Cslib/Computability/Machines/MultiTapeTuring/AddRoutine.lean
@@ -1,0 +1,96 @@
+/-
+Copyright (c) 2026 Christian Reitwiessner. All rights reserved.
+Released under Apache 2.0 license as described in the file LICENSE.
+Authors: Christian Reitwiessner
+-/
+
+module
+
+import Cslib.Foundations.Data.BiTape
+import Cslib.Foundations.Data.RelatesInSteps
+
+public import Cslib.Computability.Machines.MultiTapeTuring.Basic
+public import Cslib.Computability.Machines.MultiTapeTuring.ListEncoding
+public import Cslib.Computability.Machines.MultiTapeTuring.SuccRoutine
+public import Cslib.Computability.Machines.MultiTapeTuring.CopyRoutine
+public import Cslib.Computability.Machines.MultiTapeTuring.PushRoutine
+public import Cslib.Computability.Machines.MultiTapeTuring.PopRoutine
+public import Cslib.Computability.Machines.MultiTapeTuring.WhileCombinator
+public import Cslib.Computability.Machines.MultiTapeTuring.SequentialCombinator
+public import Cslib.Computability.Machines.MultiTapeTuring.WithTapes
+public import Cslib.Computability.Machines.MultiTapeTuring.IteCombinator
+public import Cslib.Computability.Machines.MultiTapeTuring.EqualRoutine
+
+namespace Turing
+
+namespace Routines
+
+variable [Inhabited α] [Fintype α]
+variable {k : ℕ}
+
+-- a
+-- b
+-- 0
+
+def whileCond (cond : MultiTapeTM k.succ (WithSep α)) (tm : MultiTapeTM k (WithSep α)) :
+    MultiTapeTM k.succ (WithSep α) :=
+  let k := ⟨k, by omega⟩
+  cond <;>
+  doWhile k ((pop k) <;> (tm.extend (by omega) <;> cond)) <;>
+  (pop ⟨k, by omega⟩)
+
+def not (i : Fin k.succ) := ite i (pop i <;> push i []) (pop i <;> push i [OneTwo.one])
+
+@[simp, grind =]
+theorem not_eval_list {i : Fin k.succ} {tapes : Fin k.succ → List (List OneTwo)}
+  {h_tapes_i : tapes i ≠ []} :
+  (not i).eval_list tapes = .some (Function.update tapes i (
+    (if (tapes i).head h_tapes_i = [] then [OneTwo.one] else []) :: (tapes i).tail)) := by
+  simp [not, ite_eval, h_tapes_i]
+  grind
+
+-- public def add₀ : MultiTapeTM 4 (WithSep OneTwo) :=
+--   copy 1 2 <;> push 1 []
+--   -- Here we have [a, 0 :: b, b]
+
+-- lemma add₀_eval_list {a b : List OneTwo} {ls₁ ls₂ ls₃ ls₄ : List (List OneTwo)} :
+--   add₀.eval_list
+--     [a :: ls₁, b :: ls₂, ls₃, ls₄].get =
+--     .some [a :: ls₁, [] :: b :: ls₂, b :: ls₃, ls₄].get := by
+--   simp [add₀]
+--   grind [add₀]
+
+public def add₀ : MultiTapeTM 4 (WithSep OneTwo) :=
+  (((copy 1 2 <;> push 1 []) <;>
+  -- Here we have [a, 0 :: b, b]
+  (whileCond ((eq 0 1 3) <;> not 3) (succ 1 <;> succ 2))) <;>
+  -- Here we have [a, a :: b, a + b]
+  (pop 1))
+
+@[simp, grind =]
+theorem add₀_eval_list {tapes : Fin 4 → List (List OneTwo)}
+  {h_nonempty₀ : tapes 0 ≠ []} {h_nonempty₁ : tapes 1 ≠ []} :
+  add₀.eval_list tapes = .some
+    (Function.update tapes 2 ((dya (dya_inv ((tapes 0).head h_nonempty₀) + dya_inv ((tapes 1).head h_nonempty₁)) :: (tapes 2)))) := by
+  sorry
+
+-- --- Repeatedly run a sub routine as long as a condition on the symbol
+-- --- at the first head is true.
+-- public def ite (tm₁ tm₂ : MultiTapeTM k.succ (WithSep α)) :
+--     MultiTapeTM k.succ (WithSep α) where
+--   Λ := PUnit
+--   q₀ := 0
+--   M _ syms := sorry
+
+-- @[simp]
+-- public theorem ite_eval
+--   (tm₁ tm₂ : MultiTapeTM k.succ (WithSep α))
+--   (tapes : Fin k.succ → List (List α))
+--   (h_nonempty : tapes 0 ≠ []) :
+--   (ite tm₁ tm₂).eval_list tapes =
+--     if (tapes 0).head h_nonempty = [] then tm₂.eval_list tapes else tm₁.eval_list tapes := by
+--   sorry
+
+end Routines
+
+end Turing
