Cslib/Computability/Machines/MultiTapeTuring/PopRoutine.lean
@@ -1,0 +1,47 @@
+/-
+Copyright (c) 2026 Christian Reitwiessner. All rights reserved.
+Released under Apache 2.0 license as described in the file LICENSE.
+Authors: Christian Reitwiessner
+-/
+
+module
+
+import Cslib.Foundations.Data.BiTape
+import Cslib.Foundations.Data.RelatesInSteps
+
+public import Cslib.Computability.Machines.MultiTapeTuring.Basic
+public import Cslib.Computability.Machines.MultiTapeTuring.ListEncoding
+public import Cslib.Computability.Machines.MultiTapeTuring.WithTapes
+
+-- TODO create a "common file"
+import Cslib.Computability.Machines.SingleTapeTuring.Basic
+
+namespace Turing
+
+namespace Routines
+
+variable [Inhabited α] [Fintype α]
+
+public def pop₁ : MultiTapeTM 1 (WithSep α) where
+  Λ := PUnit
+  q₀ := 0
+  M _ syms := sorry
+
+@[simp]
+public lemma pop₁_eval_list {w : List α} {ls : List (List α)} :
+  pop₁.eval_list [w :: ls].get = .some [ls].get := by
+  sorry
+
+public def pop {k : ℕ} (i : Fin k.succ) : MultiTapeTM k.succ (WithSep α) :=
+  pop₁.with_tapes #v[i] (h_le := by omega)
+
+@[simp, grind =]
+public theorem pop_eval_list {k : ℕ} {i : Fin k.succ}
+  {tapes : Fin k.succ → List (List α)}
+  {h_not_empty : tapes i ≠ []} :
+  (pop i).eval_list tapes = .some (Function.update tapes i (tapes i).tail) := by
+  sorry
+
+end Routines
+
+end Turing
