Cslib/Computability/Machines/MultiTapeTuring/SequentialCombinator.lean
@@ -15,9 +15,9 @@ public import Cslib.Computability.Machines.MultiTapeTuring.HeadStats
 
 namespace Turing
 
-namespace Routines
+namespace MultiTapeTM
 
-variable [Inhabited α] [Fintype α]
+variable [Inhabited α]
 variable {k : ℕ}
 
 --- Run tm₂ after tm₁ has terminated.
@@ -31,15 +31,23 @@ public theorem seq_eval
     tm₁.eval tapes₀ >>= fun tape₁ => tm₂.eval tape₁ := by
   sorry
 
+@[simp, grind=]
 public theorem seq_eval_list
-  (tm₁ tm₂ : MultiTapeTM k (WithSep α))
-  (tapes₀ : Fin k → List (List α)) :
+  {tm₁ tm₂ : MultiTapeTM k (WithSep α)}
+  {tapes₀ : Fin k → List (List α)} :
   (seq tm₁ tm₂).eval_list tapes₀ =
     tm₁.eval_list tapes₀ >>= fun tape₁ => tm₂.eval_list tape₁ := by
   sorry
 
+public theorem seq_associative
+  (tm₁ tm₂ tm₃ : MultiTapeTM k α)
+  (tapes₀ : Fin k → List (List α)) :
+  (seq (seq tm₁ tm₂) tm₃).eval = (seq tm₁ (seq tm₂ tm₃)).eval := by
+  sorry
+
+infix:90 " <;> " => seq
 
 
-end Routines
+end MultiTapeTM
 
 end Turing
